

Beatriz Bastos Borges

Nº 03 CT11350

Tarefa Básica

$$1. A = \begin{vmatrix} x & 1 \\ 5 & 3 \end{vmatrix}$$

$$B = \begin{vmatrix} 3 & -1 \\ x & 2 \end{vmatrix}$$

$$A \cdot A^{-1} = I_n \rightarrow B \cdot A = I_n$$

$$\begin{vmatrix} 3 & -1 \\ x & 2 \end{vmatrix} \cdot \begin{vmatrix} x & 1 \\ 5 & 3 \end{vmatrix} = \begin{vmatrix} 1 & 0 \\ 0 & 1 \end{vmatrix}$$

$$\begin{cases} 3x - 5 = 1 \\ xy + 10 = 0 \end{cases}$$

$$\begin{cases} 3 - 3 = 0 \\ y + 6 = 1 \end{cases}$$

$$3x - 5 = 1 \rightarrow x = \frac{6}{3} \rightarrow x = 2$$

$$y + 6 = 1 \rightarrow y = -5$$

$$x + y \rightarrow 2 + (-5) = \boxed{-3}$$

Alternativa C

$$2. A = \begin{vmatrix} 1 & 0 & 1 \\ K & 1 & 3 \\ 1 & K & 3 \end{vmatrix} \rightarrow \text{não tem inversa se:} \\ \text{sen determinante é} \\ \text{igual a zero.}$$

$$A = \begin{vmatrix} 1 & 0 & 1 \\ K & 1 & 3 \\ 1 & K & 3 \end{vmatrix} = 3 + K^2 - 1 - 3K \rightarrow K^2 - 3K + 2 = 0$$

$$\Delta = (-3)^2 - 4 \cdot 1 \cdot 2$$

$$\Delta = 9 - 8$$

$$\Delta = 1$$

$$K = \frac{3 \pm \sqrt{1}}{2 \cdot 1} = \frac{3 \pm 1}{2} \rightarrow K' = 2 \quad K'' = 1$$

Alternativa C

$$3. \quad A = \begin{vmatrix} 3 & 5 \\ 2 & 4 \end{vmatrix} \quad A \cdot A^{-1} = I_n$$

$$\det A = 12 - 10 = 2 \rightarrow \neq 0 \text{ e invertível}$$

$$B = A^{-1} = \begin{vmatrix} 4 & -5 \\ -2 & 3 \end{vmatrix} \div 2 = \begin{vmatrix} 2 & -\frac{5}{2} \\ -1 & \frac{3}{2} \end{vmatrix} \quad \text{Alternativa C}$$

$$4. \quad \begin{vmatrix} x & 1 & 2 \\ 3 & 1 & 2 \\ 10 & 1 & x \end{vmatrix} = x^2 + 2 \cdot 6 - 20 - 5x \rightarrow x^2 - 5x + 6 \neq 0$$

$x^2 - 5x + 6 \rightarrow \text{e invertível se } \det \neq 0$

$$\Delta = (-5)^2 - 4 \cdot 1 \cdot 6$$

$$\Delta = 25 - 24$$

$$\Delta = 1$$

$$x \neq \frac{5 \pm \sqrt{1}}{2 \cdot 1} \neq \frac{5 \pm 1}{2} \rightarrow x' \neq 3$$

$$\Delta x'' \neq 2$$

$$\{x \neq 3 \text{ e } x \neq 2\}$$

Alternativa A

$$5. A = \begin{vmatrix} -1 & -1 & 2 \\ 2 & 1 & -2 \\ 1 & 1 & -1 \end{vmatrix} = -1(-1-2) - (-1(-2-2)) + (-1(-2-1)) = 1 - 6 + 1 = -4$$

$$A = \begin{vmatrix} -1 & -1 & 2 \\ 2 & 1 & -2 \\ 1 & 1 & -1 \end{vmatrix} \quad A' = \begin{vmatrix} (-1(-2)) & (-2-(-2)) & (2-1) \\ (1-2) & (1-2) & (1-(-1)) \\ (2-2) & (2-4) & (-1-(-2)) \end{vmatrix}$$

$$A' = \begin{vmatrix} 1 & 1 & 1 \\ 1 & -1 & 0 \\ 0 & 2 & 1 \end{vmatrix} \quad \bar{A} = (A')^t = \begin{vmatrix} 1 & 1 & 6 \\ 0 & -1 & 2 \\ 1 & 0 & 1 \end{vmatrix}$$

$$A^{-1} = \frac{\bar{A}}{|A|} = \begin{vmatrix} 1 & 1 & 0 \\ 0 & -1 & 2 \\ 1 & 0 & 1 \end{vmatrix}$$

Alternativa B)

$$A + A^{-1} = \begin{vmatrix} -1 & -1 & 2 \\ 2 & 1 & -2 \\ 1 & 1 & -1 \end{vmatrix} + \begin{vmatrix} 1 & 1 & 6 \\ 0 & -1 & 2 \\ 1 & 0 & 1 \end{vmatrix} = \begin{vmatrix} 0 & 0 & 2 \\ 2 & 0 & 0 \\ 2 & 1 & 0 \end{vmatrix}$$

$$6. (X \cdot A)^t = B \rightarrow ((X \cdot A)^t)^t = B^t \rightarrow X \cdot A = B^t$$

$$X \cdot A \cdot A^{-1} = B^t \cdot A^{-1} \rightarrow X = B^t \cdot A^{-1}$$

Alternativa B)

$$7. B = \begin{vmatrix} x \\ y \end{vmatrix} \quad C = \begin{vmatrix} 4x+5y \\ 5x+6y \end{vmatrix}$$

$$A \cdot \begin{vmatrix} x \\ y \end{vmatrix} = \begin{vmatrix} 4x+5y \\ 5x+6y \end{vmatrix} \rightarrow A = \begin{vmatrix} 4 & 5 \\ 5 & 6 \end{vmatrix} = 24 - 25 = -1$$

$$A^{-1} = \begin{vmatrix} 6 & -5 \\ -5 & 4 \end{vmatrix} \div -1 \rightarrow A^{-1} = \begin{vmatrix} -6 & 5 \\ 5 & -4 \end{vmatrix} \quad \text{Alternativa D)}$$

$$8. A = \begin{vmatrix} 2 & k \\ -2 & 1 \end{vmatrix} = 2 - (-2k) \rightarrow 2 + 2k$$

$$\det A, \det A^{-1} = 1 \rightarrow (2 + 2k) \cdot (2 + 2k) = 1$$

$$4 + 4k + 4k + 4k^2 = 1 \rightarrow 4k^2 + 8k + 3 = 0$$

$$\Delta = 8^2 - 4 \cdot 4 \cdot 3$$

$$\Delta = 64 - 48$$

$$\Delta = 16$$

$$k = \frac{(-8) \pm \sqrt{16}}{2 \cdot 4} = \frac{(-8) \pm 4}{8}$$

$$\rightarrow k' = \frac{-4}{8} = -\frac{1}{2}$$

$$\rightarrow k'' = \frac{-12}{8} = -\frac{3}{2}$$

Soma dos valores de k : $-\frac{1}{2} + \left(-\frac{3}{2}\right) = -\frac{4}{2} = -2$

Alternativa B)

$$9. a) (A+B) \cdot (A-B) = A^2 - AB + BA - B^2$$

$$b) (A+B)^2 = A^2 + 2AB + B^2$$

$$\rightarrow AB = BA$$

$$c) \det A \rightarrow \det A = 1$$

$$\det(-A) = (-1)^2 \cdot \det A = \det A$$

$$\rightarrow \det(-A) = (-1)^2 \cdot \det A = \det A$$

$$d) B = A^{-1} \rightarrow \det A \cdot \det B = 1 \rightarrow \det B = \frac{1}{\det A}$$